Implement draft of character classes

extraction/Helpers.ml
@@ -21,25 +21,34 @@ let from_list ls = String.init (List.length ls) (List.nth ls)
 
 let test_regex regex input at =
   let groups = (Extracted.StaticSemantics.countLeftCapturingParensWithin regex []) in
-  let matcher = Extracted.Semantics.compilePattern regex groups in
-  let ls_input = to_list input in
+  let rer = {
+    RegExp.ignoreCase = false;
+    RegExp.multiline = false;
+    RegExp.dotAll = false;
+    RegExp.unicode = false;
+    RegExp.capturingGroupsCount = groups;
+  } in
+  match Extracted.Semantics.compilePattern regex rer with
+  | Success matcher ->
+    let ls_input = to_list input in
 
-  match matcher ls_input at with
+    (match matcher ls_input at with
 
-  | Success (Some { MatchState.endIndex = i; MatchState.captures = captures; _ }) -> 
-    assert (List.length captures == groups);
-    Printf.printf "Matched %d characters ([%d-%d]) in '%s' (length=%d)\n" (i - at) at i input (List.length ls_input);
-    let f id = 
-      match List.nth captures (id - 1) with
-      | None ->
-          Printf.printf "Group %d: undefined\n" id
-      | Some { CaptureRange.startIndex = s; CaptureRange.endIndex = e } ->
-          Printf.printf "Group %d: '%s' ([%d-%d])\n" id (from_list (drop s (take e ls_input))) s e
-    in
-    List.iter f (Extracted.List.Range.Nat.Length.range 1 groups)
+    | Success (Some { MatchState.endIndex = i; MatchState.captures = captures; _ }) -> 
+      assert (List.length captures == groups);
+      Printf.printf "Matched %d characters ([%d-%d]) in '%s' (length=%d)\n" (i - at) at i input (List.length ls_input);
+      let f id = 
+        match List.nth captures (id - 1) with
+        | None ->
+            Printf.printf "Group %d: undefined\n" id
+        | Some { CaptureRange.startIndex = s; CaptureRange.endIndex = e } ->
+            Printf.printf "Group %d: '%s' ([%d-%d])\n" id (from_list (drop s (take e ls_input))) s e
+      in
+      List.iter f (Extracted.List.Range.Nat.Length.range 1 groups)
 
-  | Success None -> Printf.printf "No match on '%s' \n" input
+    | Success None -> Printf.printf "No match on '%s' \n" input
 
-  | Failure OutOfFuel -> Printf.printf "Out of fuel on '%s' \n" input
+    | Failure OutOfFuel -> Printf.printf "Out of fuel on '%s' \n" input
 
-  | Failure AssertionFailed -> Printf.printf "Assertion error on '%s' \n" input
+    | Failure AssertionFailed -> Printf.printf "Assertion error during matching on '%s' \n" input)
+  | Failure AssertionFailed -> Printf.printf "Assertion error during compilation \n"
