extraction/Interop.ml
@@ -1,0 +1,2 @@
+let line_terminators = '\n' :: '\r' :: []
+let all_chars = List.init 128 (Char.chr)
