MECMAR/spec/ClutterFree.v
@@ -1,19 +1,30 @@
-From Warblre Require Import Result Base Patterns Notation Semantics Correctness.
+From Warblre Require Import Result Base Patterns Notation Semantics Correctness Compile.
 
-Module ClutterFree.
-  Definition regex_match (r: Regex) (rer: RegExp) (input: list Character) (start: non_neg_integer):   
-      Correctness.Groups.Ranges r 1 (RegExp.capturingGroupsCount rer) (RegExp.capturingGroupsCount rer) ->
-      0 <= start <= (length input) ->
-      option MatchState :=
-    let res0 := Semantics.compilePattern r rer input start in 
-    match res0 as res return 
-        res0 = res ->
-        Correctness.Groups.Ranges r 1 (RegExp.capturingGroupsCount rer) (RegExp.capturingGroupsCount rer) ->
-        0 <= start <= (length input) ->
-        option MatchState
+Import Result.Notations.
+Local Open Scope result_flow.
+
+(* Module ClutterFree.
+  Definition regex_compile (r: Regex) (rer: RegExp)
+      (P0: Compile.EarlyErrorsFree.Regex r):
+      { m: list Character -> non_neg_integer -> MatchResult | Semantics.compilePattern r rer = Success m } :=
+    match Semantics.compilePattern r rer as m return 
+      Semantics.compilePattern r rer = m -> { m: list Character -> non_neg_integer -> MatchResult | Semantics.compilePattern r rer = Success m }
     with
-    | Success v => fun _ _ _ => v
-    | Failure OutOfFuel => fun eq _ _ => match (Correctness.Termination.compilePattern r rer input start) eq with end
-    | Failure AssertionFailed => fun eq H0 H1 => match (Correctness.Safety.compilePattern r rer input start) H0 H1 eq with end
+    | Success v => fun eq => exist _ v eq
+    | Failure CompileError.AssertionFailed => fun eq => match (Compile.Safety.compilePattern r rer) P0 eq with end
     end eq_refl.
-End ClutterFree.
+
+  Definition regex_match (r: Regex) (rer: RegExp) (input: list Character) (start: non_neg_integer)
+      (P0: Compile.EarlyErrorsFree.Regex r)
+      (P1: Correctness.Groups.Ranges r 1 (RegExp.capturingGroupsCount rer) (RegExp.capturingGroupsCount rer))
+      (P2: 0 <= start <= (length input)):
+      { x: option MatchState | exists m, Semantics.compilePattern r rer = Success m /\ m input start = Success x } :=
+    let (m, Eq_m) := regex_compile r rer P0 in
+    match m input start as res return
+      m input start = res -> { x: option MatchState | exists m, Semantics.compilePattern r rer = Success m /\ m input start = Success x }
+    with
+    | Success v => fun eq => exist _ v (ex_intro _ m (conj Eq_m eq))
+    | out_of_fuel => fun eq => match (Correctness.Termination.compilePattern r rer input start m) Eq_m eq with end
+    | match_assertion_failed => fun eq => match (Correctness.Safety.compilePattern r rer input start m) P1 P2 Eq_m eq with end
+    end eq_refl.
+End ClutterFree. *)
