MECMAR/spec/Semantics.v
@@ -18,6 +18,9 @@ Module Semantics.
   (* These are used to wrap things into the error monad we will be using *)
   Coercion wrap_option := fun (T: Type) (t: option T) => @Success (option T) MatchError t.
   Coercion wrap_bool := fun (t: bool) => @Success bool MatchError t.
+
+  Coercion wrap_Matcher := fun (m: Matcher) => @Success Matcher CompileError m.
+  Coercion wrap_CharSet := fun (s: CharSet) => @Success CharSet CompileError s.
   Create HintDb Warblre_coercions.
   #[export]
   Hint Unfold CaptureRange_or_undefined MatchState_or_failure wrap_option wrap_bool : Warblre_coercions.
@@ -172,10 +175,10 @@ Module Semantics.
       (* l. If there exists a member a of A such that Canonicalize(rer, a) is cc, let found be true. Otherwise, let found be false. *)
       let! found =<< CharSet.exist A (fun a => Character.eqb a cc) in
       (* m. If invert is false and found is false, return failure. *)
-      if invert is false && found is false then
+      if (invert is false) && (found is false) then
         failure
       (* n. If invert is true and found is true, return failure. *)
-      else if invert is true && found is true then
+      else if (invert is true) && (found is true) then
         failure
       else
       (* o. Let cap be x's captures List. *)
@@ -237,23 +240,83 @@ Module Semantics.
       c y.
 
   (** 22.2.2.9 Runtime Semantics: CompileToCharSet *)
-  Definition compileToCharSet (self: ClassRanges) (rer: RegExp): CharSet := match self with
+
+  (** 22.2.2.9.1 CharacterRange *)
+
+  Definition characterRange (a b: CharSet): Result CharSet CompileError :=
+    (* 1. Assert: A and B each contain exactly one character. *)
+    assert! (CharSet.size a =? 1)%nat && (CharSet.size b =? 1)%nat ;
+    (* 2. Let a be the one character in CharSet A. *)
+    let! a =<< CharSet.unique a in
+    (* 3. Let b be the one character in CharSet B. *)
+    let! b =<< CharSet.unique b in
+    (* 4. Let i be the character value of character a. *)
+    let i := Character.numeric_value a in
+    (* 5. Let j be the character value of character b. *)
+    let j := Character.numeric_value b in
+    (* 6. Assert: i ≤ j. *)
+    assert! (i <=? j)%nat ;
+    (* 7. Return the CharSet containing all characters with a character value in the inclusive interval from i to j. *)
+    CharSet.range i j.
+
+  Definition compileToCharSet_ClassAtom (self: ClassAtom) (rer: RegExp): Result CharSet CompileError  := match self with
+  | SourceCharacter chr =>
+      CharSet.singleton chr
+  end.
+
+  Fixpoint compileToCharSet (self: ClassRanges) (rer: RegExp): Result CharSet CompileError := match self with
   | EmptyCR =>
       (* 1. Return the empty CharSet. *)
       CharSet.empty
-  | AtomChar c =>
-      (* 1. Return the CharSet containing the character matched by SourceCharacter. *)
-      CharSet.singleton c
+  | ClassAtomCR ca cr =>
+      (* 1. Let A be CompileToCharSet of ClassAtom with argument rer. *)
+      let! A =<< compileToCharSet_ClassAtom ca rer in
+      (* 2. Let B be CompileToCharSet of NonemptyClassRangesNoDash with argument rer. *)
+      let! B =<< compileToCharSet cr rer in
+      (* 3. Return the union of CharSets A and B. *)
+      CharSet.union A B
+  | RangeCR l h t =>
+      (* 1. Let A be CompileToCharSet of the first ClassAtom with argument rer. *)
+      let! A =<< compileToCharSet_ClassAtom l rer in
+      (* 2. Let B be CompileToCharSet of the second ClassAtom with argument rer. *)
+      let! B =<< compileToCharSet_ClassAtom h rer in
+      (* 3. Let C be CompileToCharSet of ClassRanges with argument rer. *)
+      let! C =<< compileToCharSet t rer in
+      (* 4. Let D be CharacterRange(A, B). *)
+      let! D =<< characterRange A B in
+      (* 5. Return the union of D and C. *)
+      CharSet.union D C
   end.
 
-  Fixpoint compileSubPattern (self: Regex) (ctx: RegexContext) (rer: RegExp) (direction: direction): Matcher := match self with
+
+  (** 22.2.2.8 Runtime Semantics: CompileCharacterClass *)
+
+  Module CompiledCharacterClass.
+    Record type := make {
+      charSet: CharSet;
+      invert: bool;
+    }.
+  End CompiledCharacterClass.
+  Notation compiled_character_class := CompiledCharacterClass.make.
+  Notation CompiledCharacterClass := CompiledCharacterClass.type.
+
+  Definition compileCharacterClass (self: CharClass) (rer: RegExp): Result CompiledCharacterClass CompileError := match self with
+  | NoninvertedCC crs =>
+      let! a =<< compileToCharSet crs rer in
+      Success (compiled_character_class a false)
+  | InvertedCC crs =>
+      let! a =<< compileToCharSet crs rer in
+      Success (compiled_character_class a true)
+  end.
+
+  Fixpoint compileSubPattern (self: Regex) (ctx: RegexContext) (rer: RegExp) (direction: direction): Result Matcher CompileError := match self with
   | Empty =>          (* Alternative :: [empty] *)
                       (* 1. Return a new Matcher with parameters (x, c) that captures nothing and performs the following steps when called: *)
-                      fun (x: MatchState) (c: MatcherContinuation) =>
+                      (fun (x: MatchState) (c: MatcherContinuation) =>
                         (* a. Assert: x is a MatchState. *)
                         (* b. Assert: c is a MatcherContinuation. *)
                         (* c. Return c(x). *)
-                        c x
+                        c x): Matcher
   | Char c =>
       (* 1. Let ch be the character matched by PatternCharacter. *)
       let ch := c in
@@ -261,13 +324,29 @@ Module Semantics.
       let A := CharSet.singleton c in
       (* 3. Return CharacterSetMatcher(rer, A, false, direction). *)
       characterSetMatcher rer A false direction
+  | Dot =>
+      (* 1. Let A be the CharSet of all characters. *)
+      let A := CharSet.all in
+      (* 2. If rer.[[DotAll]] is not true, then *)
+      let A := if RegExp.dotAll rer is not true
+        (* a. Remove from A all characters corresponding to a code point on the right-hand side of the LineTerminator production. *)
+        then CharSet.remove_all A CharSet.line_terminators
+        else A
+      in
+      (* 3. Return CharacterSetMatcher(rer, A, false, direction). *)
+      characterSetMatcher rer A false direction
+  | CharacterClass cc =>
+      (* 1. Let cc be CompileCharacterClass of CharacterClass with argument rer. *)
+      let! cc =<< compileCharacterClass cc rer in
+      (* 2. Return CharacterSetMatcher(rer, cc.[[CharSet]], cc.[[Invert]], direction). *)
+      characterSetMatcher rer (CompiledCharacterClass.charSet cc) (CompiledCharacterClass.invert cc) direction
   | Disjunction r1 r2 => (** 22.2.2.3 Runtime Semantics: CompileSubpattern *)
                       (* 1. Let m1 be CompileSubpattern of Alternative with arguments rer and direction. *)
-                      let m1 := compileSubPattern r1 (Disjunction_left r2 :: ctx) rer direction in
+                      let! m1 =<< compileSubPattern r1 (Disjunction_left r2 :: ctx) rer direction in
                       (* 2. Let m2 be CompileSubpattern of Disjunction with arguments rer and direction. *)
-                      let m2 := compileSubPattern r2 (Disjunction_right r1 :: ctx) rer direction in
+                      let! m2 =<< compileSubPattern r2 (Disjunction_right r1 :: ctx) rer direction in
                       (* 3. Return a new Matcher with parameters (x, c) that captures m1 and m2 and performs the following steps when called: *)
-                      fun (x: MatchState) (c: MatcherContinuation) =>
+                      (fun (x: MatchState) (c: MatcherContinuation) =>
                         (* a. Assert: x is a MatchState. *)
                         (* b. Assert: x is a MatchState. *)
                         (* c. Let r be m1(x, c). *)
@@ -277,10 +356,10 @@ Module Semantics.
                           r
                         else
                         (* e. Return m2(x, c). *)
-                        m2 x c
+                        m2 x c): Matcher
   | Quantified r qu => (** Term :: Atom Quantifier *)
                       (* 1. Let m be CompileAtom of Atom with arguments rer and direction. *)
-                      let m := compileSubPattern r  (Quantified_inner qu :: ctx) rer direction in
+                      let! m =<< compileSubPattern r  (Quantified_inner qu :: ctx) rer direction in
                       (* 2. Let q be CompileQuantifier of Quantifier. *)
                       let q := compileQuantifier qu in
                       (* 3. Assert: q.[[Min]] ≤ q.[[Max]]. *)
@@ -290,20 +369,20 @@ Module Semantics.
                       (* 5. Let parenCount be CountLeftCapturingParensWithin(Atom). *)
                       let parenCount := countLeftCapturingParensWithin r (Quantified_inner qu :: ctx) in
                       (* 6. Return a new Matcher with parameters (x, c) that captures m, q, parenIndex, and parenCount and performs the following steps when called: *)
-                      fun (x: MatchState) (c: MatcherContinuation) =>
+                      (fun (x: MatchState) (c: MatcherContinuation) =>
                         (* a. Assert: x is a MatchState. *)
                         (* b. Assert: c is a MatcherContinuation. *)
                         (* c. Return RepeatMatcher(m, q.[[Min]], q.[[Max]], q.[[Greedy]], x, c, parenIndex, parenCount). *)
-                        repeatMatcher m (CompiledQuantifier.min q) (CompiledQuantifier.max q) (CompiledQuantifier.greedy q) x c parenIndex parenCount 
+                        repeatMatcher m (CompiledQuantifier.min q) (CompiledQuantifier.max q) (CompiledQuantifier.greedy q) x c parenIndex parenCount): Matcher
   | Seq r1 r2     =>  (**  Alternative :: Alternative Term *)
                       (* 1. Let m1 be CompileSubpattern of Alternative with arguments rer and direction. *)
-                      let m1 := compileSubPattern r1 (Seq_left r2 :: ctx) rer direction in
+                      let! m1 =<< compileSubPattern r1 (Seq_left r2 :: ctx) rer direction in
                       (* 2. Let m2 be CompileSubpattern of Term with arguments rer and direction. *)
-                      let m2 := compileSubPattern r2 (Seq_right r1 :: ctx) rer direction in
+                      let! m2 =<< compileSubPattern r2 (Seq_right r1 :: ctx) rer direction in
                       (* 3. If direction is forward, then *)
                       if direction is forward then
                         (* a. Return a new Matcher with parameters (x, c) that captures m1 and m2 and performs the following steps when called: *)
-                        fun (s: MatchState) (c: MatcherContinuation) =>
+                        (fun (s: MatchState) (c: MatcherContinuation) =>
                           (* i. Assert: x is a MatchState. *)
                           (* ii. Assert: c is a MatcherContinuation. *)
                           (* iii. Let d be a new MatcherContinuation with parameters (y) that captures c and m2 and performs the following steps when called: *)
@@ -313,12 +392,12 @@ Module Semantics.
                             m2 s c
                           in
                           (* iv. Return m1(x, d). *)
-                          m1 s d
+                          m1 s d): Matcher
                       (* 4. Else, *)
                       else
                         (* a. Assert: direction is backward. *)
                         (* b. Return a new Matcher with parameters (x, c) that captures m1 and m2 and performs the following steps when called: *)
-                        fun (s: MatchState) (c: MatcherContinuation) =>
+                        (fun (s: MatchState) (c: MatcherContinuation) =>
                           (* i. Assert: x is a MatchState. *)
                           (* ii. Assert: x is a MatchState. *)
                           (* iii. Let d be a new MatcherContinuation with parameters (y) that captures c and m1 and performs the following steps when called: *)
@@ -328,14 +407,14 @@ Module Semantics.
                             m1 s c 
                           in
                           (* iv. Return m2(x, d). *)
-                          m2 s d
+                          m2 s d): Matcher
   | Group id r    =>  (**  Atom :: ( GroupSpecifier_opt Disjunction ) *)
                       (* 1.  *)
-                      let m := compileSubPattern r (Group_inner id :: ctx) rer direction in
+                      let! m =<< compileSubPattern r (Group_inner id :: ctx) rer direction in
                       (* 2. Let parenIndex be CountLeftCapturingParensBefore(Atom). *)
                       let parenIndex := countLeftCapturingParensBefore self ctx in
                       (* 3. Return a new Matcher with parameters (x, c) that captures direction, m, and parenIndex and performs the following steps when called: *)
-                      fun (x: MatchState) (c: MatcherContinuation) =>
+                      (fun (x: MatchState) (c: MatcherContinuation) =>
                         (* a. Assert: x is a MatchState. *)
                         (* b. Assert: c is a MatcherContinuation. *)
                         (* c. Let d be a new MatcherContinuation with parameters (y) that captures x, c, direction, and parenIndex and performs the following steps when called: *)
@@ -372,12 +451,12 @@ Module Semantics.
                           c z
                         in
                         (* d. Return m(x, d). *)
-                        m x d
+                        m x d): Matcher
   | Lookahead r    => (**  Assertion :: (?= Disjunction ) *)
                       (* 1. Let m be CompileSubpattern of Disjunction with arguments rer and forward. *)
-                      let m := compileSubPattern r (Lookahead_inner :: ctx) rer forward in
+                      let! m =<< compileSubPattern r (Lookahead_inner :: ctx) rer forward in
                       (* 2. Return a new Matcher with parameters (x, c) that captures m and performs the following steps when called: *)
-                      fun (x: MatchState) (c: MatcherContinuation) =>
+                      (fun (x: MatchState) (c: MatcherContinuation) =>
                         (* a. Assert: x is a MatchState. *)
                         (* b. Assert: c is a MatcherContinuation. *)
                         (* c. Let d be a new MatcherContinuation with parameters (y) that captures nothing and performs the following steps when called: *)
@@ -403,12 +482,12 @@ Module Semantics.
                         (* j. Let z be the MatchState (Input, xe, cap). *)
                         let z := match_state input xe cap in
                         (* k. Let z be the MatchState (Input, xe, cap). *)
-                        c z
+                        c z): Matcher
   | NegativeLookahead r  => (**  Assertion :: (?! Disjunction ) *)
                       (* 1. Let m be CompileSubpattern of Disjunction with arguments rer and forward. *)
-                      let m := compileSubPattern r (NegativeLookahead_inner :: ctx) rer forward in
+                      let! m =<< compileSubPattern r (NegativeLookahead_inner :: ctx) rer forward in
                       (* 2. Return a new Matcher with parameters (x, c) that captures m and performs the following steps when called: *)
-                      fun (x: MatchState) (c: MatcherContinuation) =>
+                      (fun (x: MatchState) (c: MatcherContinuation) =>
                         (* a. Assert: x is a MatchState. *)
                         (* b. Assert: c is a MatcherContinuation. *)
                         (* c. Let d be a new MatcherContinuation with parameters (y) that captures nothing and performs the following steps when called: *)
@@ -423,12 +502,12 @@ Module Semantics.
                         if r is not failure then
                           failure
                         else
-                        c x
+                        c x): Matcher
   | Lookbehind r    =>  (**  Assertion :: (?<= Disjunction ) *)
                       (* 1. Let m be CompileSubpattern of Disjunction with arguments rer and backward. *)
-                      let m := compileSubPattern r (Lookbehind_inner :: ctx) rer backward in
+                      let! m =<< compileSubPattern r (Lookbehind_inner :: ctx) rer backward in
                       (* 2. Return a new Matcher with parameters (x, c) that captures m and performs the following steps when called: *)
-                      fun (x: MatchState) (c: MatcherContinuation) =>
+                      (fun (x: MatchState) (c: MatcherContinuation) =>
                         (* a. Assert: x is a MatchState. *)
                         (* b. Assert: c is a MatcherContinuation. *)
                         (* c. Let d be a new MatcherContinuation with parameters (y) that captures nothing and performs the following steps when called: *)
@@ -454,12 +533,12 @@ Module Semantics.
                         (* j. Let z be the MatchState (Input, xe, cap). *)
                         let z := match_state input xe cap in
                         (* k. Let z be the MatchState (Input, xe, cap). *)
-                        c z
+                        c z): Matcher
   | NegativeLookbehind r  => (**  Assertion :: (?<! Disjunction ) *)
                       (* 1. Let m be CompileSubpattern of Disjunction with arguments rer and backward. *)
-                      let m := compileSubPattern r (NegativeLookbehind_inner :: ctx) rer backward in
+                      let! m =<< compileSubPattern r (NegativeLookbehind_inner :: ctx) rer backward in
                       (* 2. Return a new Matcher with parameters (x, c) that captures m and performs the following steps when called: *)
-                      fun (x: MatchState) (c: MatcherContinuation) =>
+                      (fun (x: MatchState) (c: MatcherContinuation) =>
                         (* a. Assert: x is a MatchState. *)
                         (* b. Assert: c is a MatcherContinuation. *)
                         (* c. Let d be a new MatcherContinuation with parameters (y) that captures nothing and performs the following steps when called: *)
@@ -474,7 +553,7 @@ Module Semantics.
                         if r is not failure then
                           failure
                         else
-                        c x
+                        c x): Matcher
   | BackReference de => (** AtomEscape :: DecimalEscape *)
                       (* 1. Let n be the CapturingGroupNumber of DecimalEscape. *)
                       let n := de in
@@ -488,11 +567,11 @@ Module Semantics.
       The syntax-directed operation CompilePattern takes argument rer (a RegExp Record) and returns an
       Abstract Closure that takes a List of characters and a non-negative integer and returns a MatchResult. It is
       defined piecewise over the following productions: *)
-  Definition compilePattern (r: Regex) (rer: RegExp): list Character -> non_neg_integer -> MatchResult :=
+  Definition compilePattern (r: Regex) (rer: RegExp): Result (list Character -> non_neg_integer -> MatchResult) CompileError :=
     (* 1. Let m be CompileSubpattern of Disjunction with arguments rer and forward. *)
-    let m := compileSubPattern r nil rer forward in
+    let! m =<< compileSubPattern r nil rer forward in
     (* 2. Return a new Abstract Closure with parameters (Input, index) that captures rer and m and performs the following steps when called: *)
-    fun (input: list Character) (index: non_neg_integer) =>
+    Success (fun (input: list Character) (index: non_neg_integer) =>
       (* a. Assert: Input is a List of characters. *)
       (* b. Assert: 0 ≤ index ≤ the number of elements in Input. *)
       assert! (0 <=? index)%nat && (index <=? (length input))%nat ;
@@ -507,5 +586,5 @@ Module Semantics.
       (* e. Let x be the MatchState (Input, index, cap). *)
       let x := match_state input (Z.of_nat index) cap in
       (* f. Return m(x, c). *)
-      m x c.
+      m x c).
 End Semantics.
