MECMAR/props/Compile.v
@@ -1,0 +1,124 @@
+From Coq Require Import PeanoNat ZArith Bool Lia Program.Equality List.
+From Warblre Require Import List Tactics Specialize Focus Result Base Patterns StaticSemantics Notation Semantics Definitions.
+
+Import Result.Notations.
+Import Semantics.
+
+Module Compile.
+
+  Inductive SingletonClassAtom: ClassAtom -> Character -> Prop :=
+  | Singleton_SourceCharacter: forall c, SingletonClassAtom (SourceCharacter c) c.
+
+  Module EarlyErrorsFree.
+
+    Inductive ClassRanges: Patterns.ClassRanges -> Prop :=
+    | EmptyCR: ClassRanges Patterns.EmptyCR
+    | ClassAtomCR: forall ca t, ClassRanges t -> ClassRanges (Patterns.ClassAtomCR ca t)
+    | RangeCR: forall l h cl ch t,
+        SingletonClassAtom l cl ->
+        SingletonClassAtom h ch ->
+        (Character.numeric_value cl <= Character.numeric_value ch)%nat ->
+        ClassRanges t ->
+        ClassRanges (Patterns.RangeCR l h t).
+
+    Inductive CharClass: Patterns.CharClass -> Prop :=
+    | NoninvertedCC: forall crs, ClassRanges crs -> CharClass (Patterns.NoninvertedCC crs)
+    | InvertedCC: forall crs, ClassRanges crs -> CharClass (Patterns.InvertedCC crs).
+
+    Inductive Regex: Patterns.Regex -> Prop :=
+    | Empty: Regex Patterns.Empty
+    | Char: forall chr, Regex (Patterns.Char chr)
+    | Dot: Regex Patterns.Dot
+    | CharacterClass: forall cc, CharClass cc -> Regex (Patterns.CharacterClass cc)
+    | Disjunction: forall r1 r2, Regex r1 -> Regex r2 -> Regex (Patterns.Disjunction r1 r2)
+    | Quantified: forall r q, Regex r -> Regex (Patterns.Quantified r q)
+    | Seq: forall r1 r2, Regex r1 -> Regex r2 -> Regex (Patterns.Seq r1 r2)
+    | Group: forall name r, Regex r -> Regex (Patterns.Group name r)
+    | Lookahead: forall r, Regex r -> Regex (Patterns.Lookahead r)
+    | NegativeLookahead: forall r, Regex r -> Regex (Patterns.NegativeLookahead r)
+    | Lookbehind: forall r, Regex r -> Regex (Patterns.Lookbehind r)
+    | NegativeLookbehind: forall r, Regex r -> Regex (Patterns.NegativeLookbehind r)
+    | BackReference: forall id, Regex (BackReference id).
+  End EarlyErrorsFree.
+
+  Module Safety.
+
+    Lemma compileToCharSet_ClassAtom: forall ca rer, compileToCharSet_ClassAtom ca rer <> compile_assertion_failed.
+    Proof. intros [ c ] rer. cbn. easy. Qed.
+
+    Lemma compileToCharSet_ClassAtom_singleton: forall a rer r c,
+      SingletonClassAtom a c ->
+      Semantics.compileToCharSet_ClassAtom a rer = Success r ->
+      r = c :: nil.
+    Proof.
+      induction a; intros rer c r Sing_a Eq_r; dependent destruction Sing_a.
+      cbn in Eq_r. injection Eq_r as <-. reflexivity.
+    Qed.
+
+    Lemma compileToCharSet: forall crs rer,
+      EarlyErrorsFree.ClassRanges crs ->
+      compileToCharSet crs rer <> compile_assertion_failed.
+    Proof.
+      induction crs; intros rer H; dependent destruction H; cbn.
+      - easy.
+      - specialize IHcrs with (1 := H).
+        focus § _ (_ [] _) § auto destruct; destruct f; try easy.
+        + congruence.
+        + exfalso. apply (compileToCharSet_ClassAtom _ _ AutoDest_).
+      - specialize IHcrs with (1 := H2).
+        focus § _ (_ [] _) § auto destruct; destruct f; try easy.
+        + pose proof (compileToCharSet_ClassAtom_singleton _ _ _ _ H AutoDest_) as ->.
+          pose proof (compileToCharSet_ClassAtom_singleton _ _ _ _ H0 AutoDest_0) as ->.
+          cbn in AutoDest_2. focus § _ [] _ § auto destruct in AutoDest_2.
+          boolean_simplifier. spec_reflector Nat.leb_spec0.
+          easy.
+        + exfalso. apply (IHcrs _ AutoDest_1).
+        + exfalso. apply (compileToCharSet_ClassAtom _ _ AutoDest_0).
+        + exfalso. apply (compileToCharSet_ClassAtom _ _ AutoDest_).
+    Qed.
+
+    Lemma compileCharacterClass: forall cc rer,
+      EarlyErrorsFree.CharClass cc ->
+      compileCharacterClass cc rer <> compile_assertion_failed.
+    Proof.
+      intros [ crs | crs ] rer H; dependent destruction H.
+      - cbn. focus § _ (_ [] _) § auto destruct; destruct f; try easy. exfalso. apply (compileToCharSet _ _ H AutoDest_).
+      - cbn. focus § _ (_ [] _) § auto destruct; destruct f; try easy. exfalso. apply (compileToCharSet _ _ H AutoDest_).
+    Qed.
+
+    Lemma compileSubPattern: forall r ctx rer dir,
+      EarlyErrorsFree.Regex r ->
+      compileSubPattern r ctx rer dir <> compile_assertion_failed.
+    Proof.
+      induction r; intros ctx rer dir H; dependent destruction H; cbn; try discriminate.
+      - focus § _ (_ [] _) § auto destruct; destruct f; try easy.
+        exfalso. apply (compileCharacterClass _ _ H AutoDest_).
+      - focus § _ (_ [] _) § auto destruct; destruct f; try easy.
+        + exfalso. apply IHr2 with (2 := AutoDest_0). assumption.
+        + exfalso. apply IHr1 with (2 := AutoDest_). assumption.
+      - focus § _ (_ [] _) § auto destruct. destruct f; try easy.
+        exfalso. apply IHr with (2 := AutoDest_). assumption.
+      - focus § _ (_ [] _) § auto destruct; destruct f; try easy.
+        + exfalso. apply IHr2 with (2 := AutoDest_0). assumption.
+        + exfalso. apply IHr1 with (2 := AutoDest_). assumption.
+      - focus § _ (_ [] _) § auto destruct; destruct f; try easy.
+        exfalso. apply IHr with (2 := AutoDest_). assumption.
+      - focus § _ (_ [] _) § auto destruct; destruct f; try easy.
+        exfalso. apply IHr with (2 := AutoDest_). assumption.
+      - focus § _ (_ [] _) § auto destruct; destruct f; try easy.
+        exfalso. apply IHr with (2 := AutoDest_). assumption.
+      - focus § _ (_ [] _) § auto destruct; destruct f; try easy.
+        exfalso. apply IHr with (2 := AutoDest_). assumption.
+      - focus § _ (_ [] _) § auto destruct; destruct f; try easy.
+        exfalso. apply IHr with (2 := AutoDest_). assumption.
+    Qed.
+
+    Lemma compilePattern: forall r rer,
+      EarlyErrorsFree.Regex r ->
+      compilePattern r rer <> compile_assertion_failed.
+    Proof.
+      intros r rer H. unfold compilePattern. focus § _ (_ [] _) § auto destruct; destruct f; try easy.
+      exfalso. apply (compileSubPattern _ _ _ _ H AutoDest_).
+    Qed.
+  End Safety.
+End Compile.
