extraction/Extraction.v
@@ -10,8 +10,14 @@ From Coq Require extraction.ExtrOcamlZInt.
 
 Extract Constant Character => "char".
 Extract Constant Character.eqb => "Char.equal".
+Extract Constant Character.eqs => "Char.equal".
+Extract Constant Character.numeric_value => "Char.code".
+Extract Constant Character.from_numeric_value => "Char.chr".
 
 Extract Constant GroupName => "int".
 Extract Constant GroupName.eqb => "Int.equal".
 
-Extraction "Extracted.ml" Semantics.compilePattern ClutterFree.regex_match.
+Extract Constant CharSet.line_terminators => "Interop.line_terminators".
+Extract Constant CharSet.all => "Interop.all_chars".
+
+Extraction "Extracted.ml" Semantics.compilePattern.
